Add logical AND function

ETCS_Pred.thy
@@ -53,4 +53,66 @@ lemma NOT_is_false_implies_true:
   shows "NOT \<circ>\<^sub>c p = \<f> \<Longrightarrow> p = \<t>"
   using NOT_false_is_true assms true_false_only_truth_values by fastforce
 
+subsection \<open>AND\<close>
+
+definition AND :: "cfunc" where
+  "AND = (THE \<chi>. is_pullback one one (\<Omega> \<times>\<^sub>c \<Omega>) \<Omega> (\<beta>\<^bsub>one\<^esub>) \<t> \<langle>\<t>,\<t>\<rangle> \<chi>)"
+
+lemma AND_is_pullback:
+  "is_pullback one one (\<Omega> \<times>\<^sub>c \<Omega>) \<Omega> (\<beta>\<^bsub>one\<^esub>) \<t> \<langle>\<t>,\<t>\<rangle> AND"
+  unfolding AND_def
+  using element_monomorphism characteristic_function_exists
+  by (typecheck_cfuncs, rule_tac the1I2, auto)
+
+lemma AND_type[type_rule]:
+  "AND : \<Omega> \<times>\<^sub>c \<Omega> \<rightarrow> \<Omega>"
+  using AND_is_pullback unfolding is_pullback_def square_commutes_def by auto
+
+lemma AND_true_true_is_true:
+  "AND \<circ>\<^sub>c \<langle>\<t>,\<t>\<rangle> = \<t>"
+  using AND_is_pullback unfolding is_pullback_def square_commutes_def
+  by (metis cfunc_type_def id_right_unit id_type one_unique_element)
+
+lemma AND_false_left_is_false:
+  assumes "p \<in>\<^sub>c \<Omega>"
+  shows "AND \<circ>\<^sub>c \<langle>\<f>,p\<rangle> = \<f>"
+proof (rule ccontr)
+  assume "AND \<circ>\<^sub>c \<langle>\<f>,p\<rangle> \<noteq> \<f>"
+  then have "AND \<circ>\<^sub>c \<langle>\<f>,p\<rangle> = \<t>"
+    using assms true_false_only_truth_values by (typecheck_cfuncs, blast)
+  then have "\<t> \<circ>\<^sub>c id one = AND \<circ>\<^sub>c \<langle>\<f>,p\<rangle>"
+    using assms by (typecheck_cfuncs, simp add: id_right_unit2)
+  then obtain j where j_type: "j \<in>\<^sub>c one" and j_id: "\<beta>\<^bsub>one\<^esub> \<circ>\<^sub>c j = id\<^sub>c one" and tt_j_eq_fp: "\<langle>\<t>,\<t>\<rangle> \<circ>\<^sub>c j = \<langle>\<f>,p\<rangle>"
+    using AND_is_pullback assms unfolding is_pullback_def by (typecheck_cfuncs, blast)
+  then have "j = id\<^sub>c one"
+    using id_type one_unique_element by auto
+  then have "\<langle>\<t>,\<t>\<rangle> = \<langle>\<f>,p\<rangle>"
+    by (typecheck_cfuncs, metis tt_j_eq_fp id_right_unit2)
+  then have "\<t> = \<f>"
+    using assms cart_prod_eq2 by (typecheck_cfuncs, auto)
+  then show "False"
+    using true_false_distinct by auto
+qed
+
+lemma AND_false_right_is_false:
+  assumes "p \<in>\<^sub>c \<Omega>"
+  shows "AND \<circ>\<^sub>c \<langle>p,\<f>\<rangle> = \<f>"
+proof (rule ccontr)
+  assume "AND \<circ>\<^sub>c \<langle>p,\<f>\<rangle> \<noteq> \<f>"
+  then have "AND \<circ>\<^sub>c \<langle>p,\<f>\<rangle> = \<t>"
+    using assms true_false_only_truth_values by (typecheck_cfuncs, blast)
+  then have "\<t> \<circ>\<^sub>c id one = AND \<circ>\<^sub>c \<langle>p,\<f>\<rangle>"
+    using assms by (typecheck_cfuncs, simp add: id_right_unit2)
+  then obtain j where j_type: "j \<in>\<^sub>c one" and j_id: "\<beta>\<^bsub>one\<^esub> \<circ>\<^sub>c j = id\<^sub>c one" and tt_j_eq_fp: "\<langle>\<t>,\<t>\<rangle> \<circ>\<^sub>c j = \<langle>p,\<f>\<rangle>"
+    using AND_is_pullback assms unfolding is_pullback_def by (typecheck_cfuncs, blast)
+  then have "j = id\<^sub>c one"
+    using id_type one_unique_element by auto
+  then have "\<langle>\<t>,\<t>\<rangle> = \<langle>p,\<f>\<rangle>"
+    by (typecheck_cfuncs, metis tt_j_eq_fp id_right_unit2)
+  then have "\<t> = \<f>"
+    using assms cart_prod_eq2 by (typecheck_cfuncs, auto)
+  then show "False"
+    using true_false_distinct by auto
+qed
+
 end
